tests: Rename hashmap_utils -> utils

tests/src/hashmap.rs
@@ -1,4 +1,4 @@
-//@ charon-args=--opaque=hashmap_utils
+//@ charon-args=--opaque=utils
 //@ aeneas-args=-state -split-files
 //@ [coq] aeneas-args=-use-fuel
 //@ [fstar] aeneas-args=-decreases-clauses -template-clauses
@@ -317,7 +317,7 @@ impl<T> HashMap<T> {
 }
 
 // This is a module so we can tell charon to leave it opaque
-mod hashmap_utils {
+mod utils {
     use crate::*;
 
     /// Serialize a hash map - we don't have traits, so we fix the type of the
@@ -334,11 +334,11 @@ mod hashmap_utils {
 
 pub fn insert_on_disk(key: Key, value: u64) {
     // Deserialize
-    let mut hm = hashmap_utils::deserialize();
+    let mut hm = utils::deserialize();
     // Update
     hm.insert(key, value);
     // Serialize
-    hashmap_utils::serialize(hm);
+    utils::serialize(hm);
 }
 
 /// I currently can't retrieve functions marked with the attribute #[test],
