tests/lean/Hashmap/FunsExternal.lean
@@ -6,14 +6,14 @@ open hashmap
 
 -- TODO: fill those bodies
 
-/- [hashmap::hashmap_utils::deserialize]:
+/- [hashmap::utils::deserialize]:
    Source: 'tests/src/hashmap.rs', lines 330:4-330:47 -/
-def hashmap_utils.deserialize
+def utils.deserialize
   : State → Result (State × (HashMap U64)) :=
   fun _ => .fail .panic
 
-/- [hashmap::hashmap_utils::serialize]:
+/- [hashmap::utils::serialize]:
    Source: 'tests/src/hashmap.rs', lines 325:4-325:46 -/
-def hashmap_utils.serialize
+def utils.serialize
   : HashMap U64 → State → Result (State × Unit) :=
   fun _ _ => .fail .panic
