tests/hol4/hashmap_main/hashmapMain_OpaqueScript.sml
@@ -6,10 +6,10 @@ open hashmapMain_TypesTheory
 val _ = new_theory "hashmapMain_Opaque"
 
 
-(** [hashmap_main::hashmap_utils::deserialize]: forward function *)val _ = new_constant ("hashmap_utils_deserialize_fwd",
+(** [hashmap_main::utils::deserialize]: forward function *)val _ = new_constant ("utils_deserialize_fwd",
   “:state -> (state # u64 hashmap_hash_map_t) result”)
 
-(** [hashmap_main::hashmap_utils::serialize]: forward function *)val _ = new_constant ("hashmap_utils_serialize_fwd",
+(** [hashmap_main::utils::serialize]: forward function *)val _ = new_constant ("utils_serialize_fwd",
   “:u64 hashmap_hash_map_t -> state -> (state # unit) result”)
 
 val _ = export_theory ()
